CIFC.v
@@ -7,7 +7,6 @@ Require Import Coq.Lists.List.
 
 Require Import Label.
 
-
 (* identifiers *)
 Inductive id : Type :=
   | Id : string -> id.
@@ -18,10 +17,6 @@ Inductive cn : Type :=
 
 Inductive field : Type :=
   | fd : cn -> id -> field.
-
-
-
-
 
 (* comparison of identifiers *)
 Definition beq_id x y :=
@@ -50,7 +45,7 @@ Inductive tm : Type :=
   | Skip : tm
   | Assignment : id -> tm -> tm
   | FieldWrite : tm -> id -> tm -> tm
-  | If : tm -> tm -> tm -> tm -> tm 
+  | If : id -> id -> tm -> tm -> tm 
   | Sequence : tm -> tm -> tm
   | Return : tm -> tm
 
@@ -62,30 +57,28 @@ Inductive tm : Type :=
   | v_opa_l : tm -> Label -> tm.
 
 Inductive method_def : Type :=
-  | m_def : cn -> id -> cn -> id -> tm -> method_def.
+  | m_def : cn -> id -> cn -> id -> tm -> tm -> method_def.
 
 
 Inductive CLASS : Type :=
   | class_def : cn -> (list field) -> (list method_def) -> CLASS. 
 
-
-
 Inductive value : tm -> Prop :=
   (* contants are values or normal form *)
   | v_oid :
       forall o, value (ObjId o)
-(* skip is not a terminal
+(* skip is not a terminal *)
   | v_none : 
-      value Skip *)
+      value Skip
   | v_null :
       value null
   | v_label :
       forall lb, value (l lb)
   | v_labeled : forall v lb,
-      value v ->
+     (* value v ->*)
       value (v_l v lb)
   | v_opa_labeled : forall v lb,
-      value v ->
+     (* value v ->*)
       value (v_opa_l v lb).
 
 Inductive Exception : tm -> Prop :=
@@ -126,7 +119,7 @@ Definition L_Label := LB nil.
 
 Definition empty_stack_frame : stack_frame := fun _ => None.
 Definition empty_labeled_stack_frame : labeled_stack_frame := (Labeled_frame L_Label empty_stack_frame).
-
+Definition main_labeled_stack_frame : labeled_stack_frame := (Labeled_frame L_Label empty_stack_frame).
 
 (* stack *)
 Definition stack :Type := list labeled_stack_frame.
@@ -176,17 +169,12 @@ Definition beq_oid x y :=
     | OID n1, OID n2 => if beq_nat n1 n2 then true else false
   end.
 
-
-
 Inductive Sigma := 
   | SIGMA : stack -> heap -> Sigma.
 
 Definition Config := pair Sigma tm. 
 
 Check Config.
-
-
-
 
 Definition get_stack (sgm : Sigma) : stack :=
   match sgm with
@@ -223,13 +211,11 @@ end.
 Inductive vd : Type :=
   | var_def : cn -> id -> vd.
 
-
-
 Fixpoint find_method_body (methods : list method_def) (m : id) :=
   match methods with
     | nil => None
     | h :: t =>  match h with 
-                  | m_def cls m' cls_a arg_id body => if beq_id m m' then Some (m_def cls m' cls_a arg_id body) else find_method_body t m
+                  | m_def cls m' cls_a arg_id body retV => if beq_id m m' then Some (m_def cls m' cls_a arg_id body (Return retV)) else find_method_body t m
                  end
   end.
 
@@ -237,9 +223,6 @@ Definition find_method (cls : CLASS) (m : id) :=
   match cls with
     | class_def c_name fields methods => find_method_body methods m
   end.
-
-
-
 
 Definition find_fields (cls : CLASS) := 
   match cls with
@@ -261,7 +244,6 @@ Fixpoint init_field_map (fields : list field) (fm : FieldMap) :=
   end.
 
 Check init_field_map.
-
 
 Definition add_heap_obj (h : heap) (o : oid) (ho : heapObj) :=
   fun x' => if beq_oid o x' then (Some ho) else h x'.
@@ -305,10 +287,10 @@ Inductive step : tm -> Sigma -> tm -> Sigma -> Prop :=
       value v ->
       (MethodCall v id e) / sigma ==> (MethodCall v id e') / sigma'
   (* normal method call *)
-  | ST_MethodCall3 : forall sigma sigma' o s h cls fields v lx l theta s' sf lsf arg_id cls_a body meth returnT,
+  | ST_MethodCall3 : forall sigma sigma' o s h cls fields v lx l theta s' sf lsf arg_id cls_a body meth returnT return_v,
       sigma = SIGMA s h ->
       Some (Heap_OBJ cls fields lx) = h(o) -> 
-      Some (m_def returnT meth cls_a arg_id body) = find_method cls meth -> 
+      Some (m_def returnT meth cls_a arg_id body (Return return_v)) = find_method cls meth -> 
       value v ->
       sf = sf_update (sf_update empty_stack_frame (Id "this") (ObjId o)) arg_id v ->
       l = (current_label sigma) ->
@@ -316,22 +298,22 @@ Inductive step : tm -> Sigma -> tm -> Sigma -> Prop :=
       theta = lsf -> 
       s' = cons theta s ->
       sigma' = SIGMA s' (get_heap sigma) ->
-      MethodCall (ObjId o) meth v / sigma ==> body / sigma'
+      MethodCall (ObjId o) meth v / sigma ==> (Sequence body (Return return_v)) / sigma'
   (* null pointer exception for method call *)
   | ST_MethodCallException : forall sigma v meth, 
       MethodCall null meth v / sigma ==> NPE / sigma
 
 (* method call with unlabel opaque *)
-  | ST_MethodCall_unlableOpaque : forall sigma sigma' o s h cls fields v lx l' lb s' sf lsf arg_id cls_a body meth returnT,
+  | ST_MethodCall_unlableOpaque : forall sigma sigma' o s h cls fields v lx l' lb s' sf lsf arg_id cls_a body meth returnT return_v,
       sigma = SIGMA s h ->
       Some (Heap_OBJ cls fields lx) = h(o) -> 
       sf = sf_update (sf_update empty_stack_frame (Id "this") (ObjId o)) arg_id v ->
       l' = join_label lb (current_label sigma) ->
       lsf = Labeled_frame l' sf ->
       s' = cons lsf s ->
-      Some (m_def returnT meth cls_a arg_id body) = find_method cls meth ->
+      Some (m_def returnT meth cls_a arg_id body (Return return_v)) = find_method cls meth ->
       sigma' = SIGMA s' (get_heap sigma) ->
-      MethodCall (ObjId o) meth (unlabelOpaque (v_opa_l v lb)) / sigma ==> body / sigma'
+      MethodCall (ObjId o) meth (unlabelOpaque (v_opa_l v lb)) / sigma ==> (Sequence body (Return return_v)) / sigma'
 
   (* null pointer exception for method call with unlabel opaque of null data*)
   | ST_MethodCallOpaqueDataException : forall sigma o meth, 
@@ -369,7 +351,6 @@ Inductive step : tm -> Sigma -> tm -> Sigma -> Prop :=
       (unlabel e) / sigma ==> (unlabel e') / sigma'
   (* unlabel *)
   | ST_unlabel2 : forall sigma v lb l' sigma' s h s',
-      value v ->
       sigma = SIGMA s h ->
       l' = join_label lb (current_label sigma) ->
       s' = update_current_label s l'-> 
@@ -439,6 +420,7 @@ Inductive step : tm -> Sigma -> tm -> Sigma -> Prop :=
        Assignment id e / sigma ==> Assignment id e' / sigma'
   (* assignment *)
   | ST_assignment2 : forall sigma sigma' id v s' s h,
+       value v ->
        sigma = SIGMA s h ->
        s' = update_stack_top s id v->
        sigma' = SIGMA s' h ->
@@ -449,14 +431,12 @@ Inductive step : tm -> Sigma -> tm -> Sigma -> Prop :=
   | ST_fieldWrite1 : forall sigma sigma' f e1 e1' e2,
        e1 / sigma ==>  e1' / sigma' -> 
        FieldWrite e1 f e2 / sigma ==> FieldWrite e1' f e2/ sigma'
-
   (* context rule 2 *)
-  | ST_fieldWrite2 : forall sigma sigma' f v e2 e2' t,
+  | ST_fieldWrite2 : forall sigma sigma' f v e2 e2',
+       (forall t, value t -> t<> null -> e2 <> unlabelOpaque t) ->
        value v ->
-       e2 <> unlabelOpaque t ->
        e2 / sigma ==>  e2' / sigma' -> 
        FieldWrite v f e2 / sigma ==> FieldWrite v f e2'/ sigma'
-
   (* field write normal *)
   | ST_fieldWrite3 : forall sigma sigma' o s h h' f lb cls F F' v l',
       sigma = SIGMA s h ->
@@ -465,10 +445,11 @@ Inductive step : tm -> Sigma -> tm -> Sigma -> Prop :=
       l' = join_label lb (current_label sigma) ->
       h' = add_heap_obj h o (Heap_OBJ cls F' l') ->
       sigma' = SIGMA s h' ->
+      value v->
       (FieldWrite (ObjId o) f v) / sigma ==> Skip / sigma'
   (* null pointer exception for field write *)
-  | ST_fieldWriteException : forall sigma f v o, 
-      (FieldWrite (ObjId o) f v) / sigma ==> NPE / sigma
+  | ST_fieldWriteException : forall sigma f v, 
+      (FieldWrite null f v) / sigma ==> NPE / sigma
   (* field write normal *)
   | ST_fieldWrite_opaque : forall sigma sigma' o s h h' f lo cls F F' v l' lb e2,
       e2 = unlabelOpaque (v_opa_l v lb) ->
@@ -479,6 +460,9 @@ Inductive step : tm -> Sigma -> tm -> Sigma -> Prop :=
       h' = add_heap_obj h o (Heap_OBJ cls F' l') ->
       sigma' = SIGMA s h' ->
       (FieldWrite (ObjId o) f e2) / sigma ==> Skip / sigma'
+  | ST_FieldWriteOpaqueDataException : forall sigma o f, 
+      FieldWrite (ObjId o) f (unlabelOpaque null) / sigma ==> NPE / sigma
+
 
 (* return statement *)
   (* context rule*)
@@ -496,31 +480,29 @@ Inductive step : tm -> Sigma -> tm -> Sigma -> Prop :=
        Return v / sigma ==> v / sigma'
 
 (* if statement *)
-   (* context rule 1 *)
-  | ST_if1 : forall sigma sigma' s1 s2 e1' e1 e2, 
-       e1 / sigma ==>  e1' / sigma' -> 
-       If e1 e2 s1 s2 / sigma ==> If e1' e2 s1 s2 / sigma'
-   (* context rule 2 *)
-  | ST_if2 : forall sigma sigma' s1 s2 e2' e2 v, 
-       e2 / sigma ==>  e2' / sigma' -> 
-       value v ->
-       If v e2 s1 s2 / sigma ==> If v e2' s1 s2 / sigma'
-  | ST_if_b1 : forall sigma s1 s2 v1 v2, 
+  | ST_if_b1 : forall sigma s1 s2 v1 v2 s h lsf s' lb sf id1 id2, 
+       sigma = SIGMA s h ->
+       s = cons lsf s' ->
+       lsf = Labeled_frame lb sf ->
+       Some v1 = sf(id1) ->
+       Some v2 = sf(id2) ->
        v1 = v2 ->
-       value v1 ->
-       value v2 ->
-       If v1 v2 s1 s2 / sigma ==>  s1 / sigma
-  | ST_if_b2 : forall sigma s1 s2 v1 v2, 
+       If id1 id2 s1 s2 / sigma ==>  s1 / sigma
+  | ST_if_b2 : forall sigma s1 s2 v1 v2 s h lsf s' lb sf id1 id2, 
+       sigma = SIGMA s h ->
+       s = cons lsf s' ->
+       lsf = Labeled_frame lb sf ->
+       Some v1 = sf(id1) ->
+       Some v2 = sf(id2) ->
        v1 <> v2 ->
-       value v1 ->
-       value v2 ->
-       If v1 v2 s1 s2 / sigma ==>  s2 / sigma
+       If id1 id2 s1 s2 / sigma ==>  s2 / sigma
 (* sequence *)
    (* context rule *)
   | ST_seq1 : forall sigma s1 s2 s1', 
     Sequence s1 s2 / sigma ==> Sequence s1' s2 / sigma
    (* sequence rule *)
   | ST_seq2 : forall sigma v s , 
+    value v->
     Sequence v s / sigma ==> s / sigma
 
 where "c1 '/' st '==>' c1' '/' st'" := (step c1 st c1' st').
@@ -535,22 +517,7 @@ Inductive ty : Type :=
 Definition typing_context := id -> (option ty).
 Definition empty_context : typing_context := fun _ => None.
 
-(*
-(* typing environment *)
-Reserved Notation "Gamma '|-' t '\in' T" (at level 40).
-
-Inductive has_type : typing_context -> tm -> ty -> Prop :=
-  | T_Var : forall Gamma x T,
-      Gamma x = Some T ->
-      Gamma |- Tvar x \in T
-  | T_null : forall Gamma T,
-      Gamma |- null \in T
-where "Gamma '|-' t '\in' T" := (has_type Gamma t T).
-*)
-
 Definition Class_table := cn -> option CLASS.
-
-
 
 Inductive has_type : Class_table -> typing_context -> heap -> tm -> ty -> Prop :=
 (*variable *)
@@ -568,12 +535,13 @@ Inductive has_type : Class_table -> typing_context -> heap -> tm -> ty -> Prop :
       type_of_field fields_def f = Some cls' ->
       has_type CT Gamma h (FieldAccess e f) (classTy cls')
 (* method call *)
-  | T_MethodCall : forall Gamma e meth argu CT h T returnT cls_def body arg_id arguT para_T cls_a,
+  | T_MethodCall : forall Gamma e meth argu CT h T returnT cls_def body arg_id arguT para_T cls_a returnV,
       has_type CT Gamma h e (classTy T) ->
       has_type CT Gamma h argu arguT ->
       Some cls_def = CT(T) ->
-      find_method cls_def meth = Some (m_def returnT meth cls_a arg_id body)  ->
+      find_method cls_def meth = Some (m_def returnT meth cls_a arg_id body (Return returnV))  ->
       arguT = para_T ->
+      has_type CT Gamma h (returnV) (classTy returnT) ->
       has_type CT Gamma h (MethodCall e meth argu) (classTy returnT)
 (* new exp *)
   | T_NewExp : forall h Gamma cn CT cls_def,
@@ -604,8 +572,8 @@ Inductive has_type : Class_table -> typing_context -> heap -> tm -> ty -> Prop :
       has_type CT Gamma h e T ->
       has_type CT Gamma h (opaqueCall e) (OpaqueLabeledTy T)
 (* Skip *)
-  | T_skip : forall h Gamma CT T,
-      has_type CT Gamma h Skip T
+  | T_skip : forall h Gamma CT,
+      has_type CT Gamma h Skip voidTy
 (* assignment *)
   | T_assignment : forall h Gamma CT e T x,
       Gamma x = Some T ->
@@ -619,12 +587,12 @@ Inductive has_type : Class_table -> typing_context -> heap -> tm -> ty -> Prop :
       type_of_field (find_fields cls_def) f = Some cls' ->
       has_type CT Gamma h (FieldWrite x f e) (classTy cls')
 (* if *)
-  | T_if : forall Gamma h CT e e1 e2 e3 T T',
-      has_type CT Gamma h e T ->
-      has_type CT Gamma h e1 T ->
-      has_type CT Gamma h e2 T' ->
-      has_type CT Gamma h e3 T' ->
-      has_type CT Gamma h (If e e1 e2 e3) T'
+  | T_if : forall Gamma h CT id1 id2 s1 s2 T T',
+      Gamma id1 = Some (classTy T) ->
+      Gamma id2 = Some (classTy T) ->
+      has_type CT Gamma h s1 T' ->
+      has_type CT Gamma h s2 T' ->
+      has_type CT Gamma h (If id1 id2 s1 s2) T'
 (* sequence *)
   | T_sequence : forall h Gamma CT e1 e2 T T',
       has_type CT Gamma h e1 T ->
@@ -633,15 +601,17 @@ Inductive has_type : Class_table -> typing_context -> heap -> tm -> ty -> Prop :
 (* return *)
   | T_return : forall h Gamma CT e T,
       has_type CT Gamma h e T ->
+      T <> voidTy ->
       has_type CT Gamma h (Return e) T
 (* ObjId *)
   | T_ObjId : forall h Gamma CT o cls_name F lo cls_def,
       Some cls_def = CT(cls_name) ->
       h(o) = Some (Heap_OBJ cls_def F lo) ->
       has_type CT Gamma h (ObjId o) (classTy cls_name)
-(* NPE *)
+(* NPE 
   | T_NPE : forall h Gamma CT T,
-      has_type CT Gamma h NPE T
+      has_type CT Gamma h NPE T 
+*)
 (* runtime labeled data *)
   | T_v_l : forall h Gamma lb CT v T,
       has_type CT Gamma h (l lb)  LabelTy ->
@@ -769,19 +739,19 @@ Fixpoint variable_exists (s : stack) (x : id) :=
   end.
 
 Inductive wfe_stack_frame : heap -> labeled_stack_frame -> Prop :=
-  | stack_frame_wfe : forall h lsf sf x v o lb cls_def F lo,
+  | stack_frame_wfe : forall h lsf sf o lb cls_def F lo,
         lsf = Labeled_frame lb sf ->
-        sf x = Some v ->
-        v = null \/ ((v = ObjId o) -> h(o) = Some (Heap_OBJ cls_def F lo)) \/ v = l lb ->
+        (forall x v, sf x = Some v ->
+        v = null \/ ((v = ObjId o) /\ h(o) = Some (Heap_OBJ cls_def F lo)) \/ v = l lb) ->
         wfe_stack_frame h lsf. 
 
 
 Inductive wfe_stack : Class_table -> typing_context -> heap -> stack -> Prop :=
-  | empty_stack_wfe : forall ct gamma h,
+  | main_stack_wfe : forall ct gamma h,
         wfe_heap ct gamma h -> 
         h = empty_heap ->
         gamma = empty_context -> 
-        wfe_stack ct gamma h nil
+        wfe_stack ct gamma h (cons main_labeled_stack_frame nil)
   | stack_wfe : forall s ct h gamma x T s' lb sf cls_def gamma' v v', 
         s = cons (Labeled_frame lb sf) s'->
         wfe_stack ct gamma h s' ->
@@ -794,6 +764,29 @@ Inductive wfe_stack : Class_table -> typing_context -> heap -> stack -> Prop :=
         gamma'= (fun x' => if beq_id x x' then (Some (classTy T)) else (gamma x)) ->
         ct T = Some cls_def -> 
         wfe_stack ct gamma' h s.
+
+Lemma beq_equal : forall x x', beq_id x x' = true -> x' = x.
+Proof.
+   intros. unfold beq_id in H. 
+  destruct x. destruct x'.  f_equal.
+ case_eq (string_dec s s0). 
+  - intros. rewrite -> e. auto.
+  - intro. intro. rewrite -> H0 in H. inversion H. 
+Qed.
+
+Lemma Typed_variable : forall sigma s h ct gamma x T sf s' lb,
+  sigma = SIGMA s h ->
+  wfe_stack ct gamma h s ->
+   gamma x = Some T -> 
+   s = cons (Labeled_frame lb sf) s' -> 
+   exists v, sf x = Some v.
+Proof with eauto.
+  intros. inversion H0.
+  + subst. inversion H1. 
+  + subst. case_eq (beq_id x0 x). intros. rewrite -> H in H1. inversion H1. subst. - exists v. rewrite <- H9. 
+        inversion H3. subst. f_equal. apply beq_equal. assumption.
+ - intros. rewrite -> H in H1. rewrite -> H7 in H1. inversion H1.  
+Qed.
 
 Inductive wfe : Class_table -> typing_context -> Sigma -> Prop :=
   | wfe_sigma : forall sigma s h ct gamma ,
@@ -816,30 +809,6 @@ Proof with eauto.
 Qed. 
 
 Check f_equal.
-
-Lemma beq_equal : forall x x', beq_id x x' = true -> x' = x.
-Proof.
-   intros. unfold beq_id in H. 
-  destruct x. destruct x'.  f_equal.
- case_eq (string_dec s s0). 
-  - intros. rewrite -> e. auto.
-  - intro. intro. rewrite -> H0 in H. inversion H. 
-Qed.
-
-Lemma Typed_variable : forall sigma s h ct gamma x T lb sf s',
-  sigma = SIGMA s h ->
-  wfe_stack ct gamma h s ->
-   gamma x = Some T -> 
-   s = cons (Labeled_frame lb sf) s' -> 
-   exists v, sf x = Some v.
-Proof with eauto.
-  intros. inversion H0.
-  + subst. inversion H9.
-  + subst. case_eq (beq_id x0 x). intros. rewrite -> H in H1. inversion H1. subst. - exists v. rewrite <- H9. 
-        inversion H3. subst. f_equal. apply beq_equal. assumption.
- - intros. rewrite -> H in H1. rewrite -> H7 in H1. inversion H1.  
-Qed.
-
 
 Lemma wfe_oid : forall o ct gamma s h sigma cls_def cn, 
   sigma = SIGMA s h ->
@@ -912,6 +881,14 @@ right. intro.  intros contra. inversion contra.
 Qed.
 
 
+Lemma stack_not_nil : forall sigma gamma CT s h, 
+  sigma = SIGMA s h ->  wfe_heap CT gamma h -> wfe_stack CT gamma h s -> exists lsf s', s = cons lsf s'.
+Proof with auto.
+  intros. inversion H1. exists main_labeled_stack_frame. exists nil. auto. 
+  exists (Labeled_frame lb sf). exists s'. auto. 
+Qed.
+ 
+
 Theorem progress : forall t T sigma gamma CT s h, 
   sigma = SIGMA s h ->  wfe_heap CT gamma h -> wfe_stack CT gamma h s -> 
   has_type CT gamma h t T -> value t \/ exists t' sigma', t / sigma ==> t' / sigma'.
@@ -953,16 +930,18 @@ Proof with auto.
             (sigma:=sigma) (sigma':=sigma') (o:=o) (s:=s) (h:=h) (fname:=f) (lb:=lb) 
             (cls:=cls_def) (fields:=F) (v:=v) (l':=l') (s':=s'). 
             auto. auto. auto.            auto. auto. auto. 
+    (* skip *)
+    rewrite <- H7 in H2. inversion H2. 
     (* call field access on null point object *)
     exists NPE. exists sigma. apply ST_fieldReadException.
     (* label is primitive: calling field access is not valid *)
     rewrite <- H7 in H2. inversion H2.
    
      (* call field access on labeled value*)
-    {rewrite <- H8  in H2. inversion H2. }
+    {rewrite <- H7  in H2. inversion H2. }
     
      (* call field access on opaque label value*)
-    {rewrite <- H8  in H2. inversion H2. }
+    {rewrite <- H7  in H2. inversion H2. }
 
      (* context rule *)
     + { destruct H6 as [e']. destruct H6 as [sigma'].
@@ -981,11 +960,11 @@ Proof with auto.
             remember (Labeled_frame l sf) as lsf. 
             remember (cons lsf s) as s'.
             remember (SIGMA s' (get_heap sigma)) as sigma'.
-            exists body. exists sigma'.
+            exists (Sequence body (Return returnV)) . exists sigma'.
             apply ST_MethodCall3 with (sigma:=sigma) (sigma':=sigma') (o:=o) (s:=s) (h:=h) (cls:=cls_def) (fields:=F) 
                                        (v:=argu) (lx:=lo) (l:=l) 
                                        (theta:=lsf) (s':=s') (sf:=sf) (lsf:=lsf) (arg_id:=arg_id) 
-                                        (cls_a:=cls_a) (body:=body) (meth:=meth) (returnT:=returnT); auto.
+                                        (cls_a:=cls_a) (body:=body) (meth:=meth) (returnT:=returnT) (return_v:=returnV); auto.
             rewrite <- H12 in H2. inversion H2. rewrite <- H13; auto. 
           (* case analysis for argument, if the argument is not a value *)
             subst. 
@@ -1001,7 +980,7 @@ Proof with auto.
                                             (v:=(ObjId o)) (e:=unlabelOpaque t) (e':=unlabelOpaque e') (id:=meth).
                   intros. subst. intro contra. inversion contra. rewrite -> H9 in H. inversion H4.
                       rewrite <- H8 in H; subst; inversion H7. auto.  subst. inversion H7.  subst.
-                      inversion H7. subst. inversion H7.   
+                      inversion H7. subst. inversion H7. subst. inversion H7. subst. inversion H7.
                       assumption. apply v_oid. 
                       subst. 
                       remember (SIGMA s h ) as sigma.
@@ -1010,11 +989,11 @@ Proof with auto.
                       remember (Labeled_frame l' sf) as lsf. 
                       remember (cons lsf s) as s'.
                       remember (SIGMA s' (get_heap sigma)) as sigma''.
-                      exists body. exists sigma''. 
+                      exists (Sequence body (Return returnV)). exists sigma''. 
                       apply ST_MethodCall_unlableOpaque with (sigma:=sigma) (sigma':=sigma'') (o:=o) (s:=s) (h:=h) 
                                             (cls:=cls_def0) (fields:=F) (v:=t') (lx:=lo) (l':=l') (lb:=lb) (s':=s')
                                            (sf:=sf) (lsf:=lsf) (arg_id:=arg_id) (cls_a:=cls_a) (body:=body) 
-                                           (meth:=meth) (returnT:=returnT).
+                                           (meth:=meth) (returnT:=returnT) (return_v:=returnV).
                       auto. auto. auto. auto. auto. auto. subst. 
                       rewrite <- H12 in H2. inversion H2. rewrite <- H6. rewrite -> H3; auto. 
                       auto.
@@ -1029,12 +1008,15 @@ Proof with auto.
                   intro. intro. intro. 
 
                   assert (argu <> unlabelOpaque t).  apply (H4 t). apply (H4 t). auto. apply v_oid.
+                    
+                  rewrite <- H6 in H2_. inversion H2_.
+      
                   (* case for argu <> unlabelOpaque t exception *)
                   subst. exists NPE. exists (SIGMA s h). 
               apply ST_MethodCallException with (sigma:=(SIGMA s h)) (v:=argu) (meth:=meth).
 
                   subst. inversion H2_.
-                rewrite <- H7 in H2_. inversion H2_.                 rewrite <- H7 in H2_. inversion H2_. 
+                rewrite <- H6 in H2_. inversion H2_.                 rewrite <- H6 in H2_. inversion H2_. 
       +  destruct H5 as [t']. destruct H5 as [sigma']. exists (MethodCall t' meth argu). exists (sigma').   
                   apply ST_MethodCall1 with (sigma:=sigma) (sigma':=sigma') (e2:=argu) (e:=e) (e':=t') (id:=meth). apply H5.
 
@@ -1109,6 +1091,7 @@ Proof with auto.
             destruct IHhas_type. auto. auto. auto. 
              (* subgoal #1 *)
                 + inversion H3. rewrite <- H4 in H2. inversion H2. 
+                     rewrite <- H4 in H2.  inversion H2. 
                     exists NPE. exists sigma.  apply ST_unlabelDataException with (sigma:=sigma).
                     rewrite <- H4 in H2.  inversion H2. 
 
@@ -1121,7 +1104,7 @@ Proof with auto.
                 auto. auto. auto. auto. auto.
 
             (* subgoal #3 *)
-                rewrite <- H5 in H2.  inversion H2. 
+                rewrite <- H4 in H2.  inversion H2. 
 
              (* subgoal #4 *)
                 + destruct H3 as [t']. destruct H3 as [sigma']. 
@@ -1133,12 +1116,13 @@ Proof with auto.
          destruct IHhas_type. auto. auto. auto. 
             (* subgoal #1 *)
                 + inversion H3. rewrite <- H4 in H2. inversion H2. 
+                    rewrite <- H4 in H2. inversion H2. 
                     exists NPE. exists sigma.  apply ST_labelOfDataException with (sigma:=sigma).
                     rewrite <- H4 in H2.  inversion H2.
                     
                    exists (l lb). exists (sigma). apply ST_labelof2 with (v:=v) (lb:=lb).
 
-                    rewrite <- H5 in H2. inversion H2. 
+                    rewrite <- H4 in H2. inversion H2. 
              (* subgoal #2 *)
                 + destruct H3 as [t']. destruct H3 as [sigma']. 
                     exists  (labelOf t'). exists sigma'. apply ST_labelof1 with (sigma:=sigma) (sigma':=sigma') (e:=e) (e':=t'). auto. 
@@ -1148,10 +1132,11 @@ Proof with auto.
          destruct IHhas_type. auto. auto. auto. 
             (* subgoal #1 *)
                 + inversion H3. rewrite <- H4 in H2. inversion H2. 
+                    rewrite <- H4 in H2. inversion H2. 
                     exists NPE. exists sigma.  apply ST_unlabel_opaqueDataException with (sigma:=sigma).
                     rewrite <- H4 in H2.  inversion H2.
               
-                     rewrite <- H5 in H2. inversion H2. 
+                     rewrite <- H4 in H2. inversion H2. 
  
                 remember ( join_label lb (current_label sigma)) as l'.
                 remember (update_current_label s l') as s'.
@@ -1200,102 +1185,362 @@ Proof with auto.
                   exists (opaqueCall(t') ). exists sigma'.
                   apply ST_opaquecall1 with (sigma:=(SIGMA s h)) (sigma':=sigma') (e:= Return (NewExp c) ) (e':= t').
                   intros. intro contra. inversion contra. rewrite <- H5 in H3.  inversion H3.         auto.
-                  (* return label *)
+                  (* return label : when e <> return v*)
+                  subst. 
+                  remember (SIGMA s h)  as sigma. 
+                  assert (exists lsf s', s = cons lsf s'). apply stack_not_nil with (sigma:=(SIGMA s h)) (s:=s) (h:=h) (gamma:=Gamma) (CT:=CT).
+                  auto. auto. auto. 
+                  destruct H3 as [lsf].  destruct H3 as [s'].
+                  remember (current_label sigma) as lb. 
+                  remember (SIGMA s' h) as sigma''.
+                  exists (v_opa_l (l l0) lb). exists sigma''. 
+                  apply ST_opaquecall_return2 with (sigma:=sigma) (sigma':=sigma'') (s:=s) (h:=h) (lb:=lb) (s':=s') (lsf:=lsf) (v:=(l l0)). 
+                  auto. auto. auto. auto. apply v_label. 
+                  
+                  
                   subst. 
                   exists (opaqueCall(t') ). exists sigma'.
-                  apply ST_opaquecall1 with (sigma:=(SIGMA s h)) (sigma':=sigma') (e:= Return (NewExp c) ) (e':= t').
+                  apply ST_opaquecall1 with (sigma:=(SIGMA s h)) (sigma':=sigma') (e:= Return (labelData t l0) ) (e':= t').
                   intros. intro contra. inversion contra. rewrite <- H5 in H3.  inversion H3.         auto.
 
+                  subst. 
+                  exists (opaqueCall(t') ). exists sigma'.
+                  apply ST_opaquecall1 with (sigma:=(SIGMA s h)) (sigma':=sigma') (e:= Return (unlabel t) ) (e':= t').
+                  intros. intro contra. inversion contra. rewrite <- H5 in H3.  inversion H3.         auto.
 
-    destruct H3 as [t].
-                  destruct t.
-                  rewrite -> H3 in H. 
-                  inversion H.  subst. 
-                  exists (opaqueCall(Return e')). exists sigma'.
-                  apply ST_opaquecall_return1 with (sigma:=(SIGMA s h)) (sigma':=sigma') (e:= (Tvar i)) (e':= e').
+                  subst. 
+                  exists (opaqueCall(t') ). exists sigma'.
+                  apply ST_opaquecall1 with (sigma:=(SIGMA s h)) (sigma':=sigma') (e:= Return (labelOf t) ) (e':= t').
+                  intros. intro contra. inversion contra. rewrite <- H5 in H3.  inversion H3.         auto.
+
+                  subst. 
+                  exists (opaqueCall(t') ). exists sigma'.
+                  apply ST_opaquecall1 with (sigma:=(SIGMA s h)) (sigma':=sigma') (e:= Return (unlabelOpaque t) ) (e':= t').
+                  intros. intro contra. inversion contra. rewrite <- H5 in H3.  inversion H3.         auto.
+
+                  subst. 
+                  exists (opaqueCall(t') ). exists sigma'.
+                  apply ST_opaquecall1 with (sigma:=(SIGMA s h)) (sigma':=sigma') (e:= Return (opaqueCall t) ) (e':= t').
+                  intros. intro contra. inversion contra. rewrite <- H5 in H3.  inversion H3.         auto.
+
+                   rewrite -> H3 in H2. inversion H2. inversion H5. rewrite -> H15 in H9. intuition.
+
+                  subst. 
+                  exists (opaqueCall(t') ). exists sigma'.
+                  apply ST_opaquecall1 with (sigma:=(SIGMA s h)) (sigma':=sigma') (e:= Return (Assignment i t) ) (e':= t').
+                  intros. intro contra. inversion contra. rewrite <- H5 in H3.  inversion H3.         auto.
+
+                  subst. 
+                  exists (opaqueCall(t') ). exists sigma'.
+                  apply ST_opaquecall1 with (sigma:=(SIGMA s h)) (sigma':=sigma') (e:= Return (FieldWrite t1 i t2)) (e':= t').
+                  intros. intro contra. inversion contra. rewrite <- H5 in H3.  inversion H3.         auto.
+
+                  subst. 
+                  exists (opaqueCall(t') ). exists sigma'.
+                  apply ST_opaquecall1 with (sigma:=(SIGMA s h)) (sigma':=sigma') (e:= Return (If i i0 t1 t2)) (e':= t').
+                  intros. intro contra. inversion contra. rewrite <- H5 in H3.  inversion H3.         auto.
+
+                  subst. 
+                  exists (opaqueCall(t') ). exists sigma'.
+                  apply ST_opaquecall1 with (sigma:=(SIGMA s h)) (sigma':=sigma') (e:= Return (Sequence t1 t2)) (e':= t').
+                  intros. intro contra. inversion contra. rewrite <- H5 in H3.  inversion H3.         auto.
+
+                  subst. 
+                  exists (opaqueCall(t') ). exists sigma'.
+                  apply ST_opaquecall1 with (sigma:=(SIGMA s h)) (sigma':=sigma') (e:= Return (Return t)) (e':= t').
+                  intros. intro contra. inversion contra. rewrite <- H5 in H3.  inversion H3.         auto.
+
+                  subst. 
+                  remember (SIGMA s h)  as sigma. 
+                  assert (exists lsf s', s = cons lsf s'). apply stack_not_nil with (sigma:=(SIGMA s h)) (s:=s) (h:=h) (gamma:=Gamma) (CT:=CT).
+                  auto. auto. auto. 
+                  destruct H3 as [lsf].  destruct H3 as [s'].
+                  remember (current_label sigma) as lb. 
+                  remember (SIGMA s' h) as sigma''.
+                  exists (v_opa_l (ObjId o) lb). exists sigma''. 
+                  apply ST_opaquecall_return2 with (sigma:=sigma) (sigma':=sigma'') (s:=s) (h:=h) (lb:=lb) (s':=s') (lsf:=lsf) (v:=(ObjId o)). 
+                  auto. auto. auto. auto. apply v_oid. 
+
+                  rewrite -> H3 in H2. inversion H2. inversion H5. 
+
+                  subst. 
+                  inversion H. inversion H4.
+
+                  subst. 
+                  remember (SIGMA s h)  as sigma. 
+                  remember (current_label sigma) as lb. 
+                  remember (SIGMA s' h) as sigma'.
+                  exists (v_opa_l (v_l t l0) lb). exists sigma'. 
+                  apply ST_opaquecall_return2 with (sigma:=sigma) (sigma':=sigma') (s:=s) (h:=h) (lb:=lb) (s':=s') (lsf:=lsf) (v:=(v_l t l0)). 
+                  auto. rewrite -> H5 in Heqsigma. inversion Heqsigma. auto. auto. auto. auto. 
+
+
+                  subst. inversion H. inversion H4.
+
+                  subst. 
+                  remember (SIGMA s h)  as sigma. 
+                  remember (current_label sigma) as lb. 
+                  remember (SIGMA s' h) as sigma'.
+                  exists (v_opa_l (v_opa_l t l0) lb). exists sigma'. 
+                  apply ST_opaquecall_return2 with (sigma:=sigma) (sigma':=sigma') (s:=s) (h:=h) (lb:=lb) (s':=s') (lsf:=lsf) (v:=(v_opa_l t l0)). 
+                  auto. rewrite -> H5 in Heqsigma. inversion Heqsigma. auto. auto. auto. auto. 
+                  
+                  (* return label *)
+
+                  exists (opaqueCall(t')). exists sigma'. apply ST_opaquecall1 with (sigma:=(SIGMA s h)) (sigma':=sigma') (e:=e) (e':=t'). 
+                  intros. intro contra. rewrite -> contra in H3. apply H3 with (t:=v). auto. auto.
+
+(* Skip *)
+  - left. apply v_none. 
+
+(* assignment *)
+- right. destruct IHhas_type. auto. auto. auto.
+                  remember (update_stack_top s x e) as s'.
+                  remember (SIGMA s' h) as sigma'.
+                  exists Skip. exists sigma'.
+                  apply ST_assignment2 with (sigma:=sigma) (sigma':=sigma') (id:=x) (v:=e) (s':=s') (s:=s) (h:=h).
+                  auto. auto. auto. auto.
+
+                  destruct H4 as [t']. destruct H4 as [sigma'].
+                  exists (Assignment x t'). exists sigma'. 
+                  apply ST_assignment1 with (sigma:=sigma) (sigma':=sigma') (e:=e) (e':=t') (id:=x).
                   auto. 
 
-
-
-
-
-                  apply ST_var with (id:=i) (sigma:=sigma) (s:=s) (h:=h) (lb) sf lsf v s',
-
-                  rewrite -> H3 in H.
-                  case (value t).
-                  inversion t. 
- 
- inversion H. subst. 
-                  exists (opaqueCall(Return e')).
+(* FieldWrite *)
+-right. 
+      destruct IHhas_type1. auto. auto. auto. 
+       + inversion H4. 
+          (* case analysis for argument: if the argument is a value *)
+             destruct IHhas_type2. auto. auto. auto. subst. 
+            assert (exists fieldsMap lb, h(o) = Some (Heap_OBJ cls_def fieldsMap lb)).
+            remember (SIGMA s h ) as sigma.
+            apply wfe_oid with (o:=o) (ct:=CT) (gamma:=Gamma) (s:=s) (h:=h) 
+                          (sigma:=sigma) (cls_def:=cls_def) (cn:=clsT). auto. auto. auto. auto.
+            destruct H as [F]. destruct H as [lb]. 
+            remember (SIGMA s h ) as sigma.
+            remember (join_label lb (current_label sigma)) as l'. 
+            remember (fields_update F f e) as F'. 
+            remember (add_heap_obj h o (Heap_OBJ cls_def F' l')) as h'.
+            remember (SIGMA s h') as sigma'.
+            exists Skip. exists sigma'.
+            apply ST_fieldWrite3 with (sigma:=sigma) (sigma':=sigma') (o:=o) (s:=s) (h:=h) (h':=h') (f:=f) 
+                                                      (lb:=lb) (cls:=cls_def) (F:=F) (F':=F') (v:=e) (l':=l').
+            auto. auto. auto. auto. auto. auto.  auto.
+            
+          (* case analysis for argument, if the argument is not a value *)
+            subst. 
+                destruct H6 as [t']. destruct H as [sigma'].
+                pose proof (excluded_middle_opaqueLabel e).
+                destruct H5.
+                  (* case for e = unlabelOpaque t *)
+                  destruct H5 as [t]. 
+                  rewrite -> H5 in H. inversion H. subst. 
+                  exists (FieldWrite (ObjId o) f (unlabelOpaque e')).
                   exists (sigma').
-                  apply ST_opaquecall_return1 with (sigma:=(SIGMA s h)) (sigma':=sigma') 
-                                            (e:=t) (e':=e'). auto.
-      
-                  subst. 
- 
-                  intros. subst. intro contra. inversion contra. rewrite -> H9 in H. inversion H4.
+                  apply ST_fieldWrite2 with (sigma:=(SIGMA s h)) (sigma':=sigma') 
+                                            (v:=(ObjId o)) (e2:=unlabelOpaque t) (e2':=unlabelOpaque e') (f:=f).
+                  intros. subst. intro contra. inversion contra. rewrite -> H9 in H. inversion H5.
                       rewrite <- H8 in H; subst; inversion H7. auto.  subst. inversion H7.  subst.
-                      inversion H7. subst. inversion H7.   
-                      assumption. apply v_oid. 
+                      inversion H7. subst. inversion H7. subst. inversion H7. subst. inversion H7.
+                      assumption. assumption. 
                       subst. 
+                      assert (exists fieldsMap lb, h(o) = Some (Heap_OBJ cls_def fieldsMap lb)).
                       remember (SIGMA s h ) as sigma.
-                      remember (sf_update (sf_update empty_stack_frame (Id "this") (ObjId o)) arg_id t') as sf.
-                      remember (join_label lb (current_label sigma)) as l'. 
-                      remember (Labeled_frame l' sf) as lsf. 
-                      remember (cons lsf s) as s'.
-                      remember (SIGMA s' (get_heap sigma)) as sigma''.
-                      exists body. exists sigma''. 
-                      apply ST_MethodCall_unlableOpaque with (sigma:=sigma) (sigma':=sigma'') (o:=o) (s:=s) (h:=h) 
-                                            (cls:=cls_def0) (fields:=F) (v:=t') (lx:=lo) (l':=l') (lb:=lb) (s':=s')
-                                           (sf:=sf) (lsf:=lsf) (arg_id:=arg_id) (cls_a:=cls_a) (body:=body) 
-                                           (meth:=meth) (returnT:=returnT).
-                      auto. auto. auto. auto. auto. auto. subst. 
-                      rewrite <- H12 in H2. inversion H2. rewrite <- H6. rewrite -> H3; auto. 
-                      auto.
+                      apply wfe_oid with (o:=o) (ct:=CT) (gamma:=Gamma) (s:=s) (h:=h) 
+                                    (sigma:=sigma) (cls_def:=cls_def) (cn:=clsT). auto. auto. auto. auto.
+                      destruct H5 as [F]. destruct H5 as [lo]. 
+
+                      remember (SIGMA s h ) as sigma.
+                      remember (join_label lo lb) as l'. 
+                      remember (fields_update F f t') as F'. 
+                      remember (add_heap_obj h o (Heap_OBJ cls_def F' l')) as h'.
+                      remember (SIGMA s h') as sigma'.
+                      exists Skip. exists sigma'.
+                      apply ST_fieldWrite_opaque with (sigma:=sigma) (sigma':=sigma') (o:=o) (s:=s) (h:=h) (h':=h') (f:=f) 
+                                                      (lb:=lb) (lo:=lo) (cls:=cls_def) (F:=F) (F':=F') (v:=t') (l':=l').
+                      auto. auto. auto. auto. auto. auto.  auto.
+
                   (*exception case *)
                   subst. exists NPE. exists (SIGMA s h).
-                  apply ST_MethodCallOpaqueDataException with (sigma:=(SIGMA s h)) (o:=o).  
+                  apply ST_FieldWriteOpaqueDataException with (sigma:=(SIGMA s h)) (o:=o) (f:=f).
 
                   (* case for argu <> unlabelOpaque t *)
-                  exists (MethodCall (ObjId o) meth t'). exists sigma'. 
-                  apply ST_MethodCall2 with (sigma:=(SIGMA s h)) (sigma':=sigma') (v:=((ObjId o))) 
-                                            (e:=argu) (e':=t') (id:=meth).
-                  intro. intro. intro. 
+                  exists (FieldWrite (ObjId o) f t'). exists sigma'. 
+                  apply ST_fieldWrite2 with (sigma:=(SIGMA s h)) (sigma':=sigma') (v:=((ObjId o))) 
+                                            (e2:=e) (e2':=t') (f:=f).
+                  intros. apply H5. apply v_oid. assumption.
+                  rewrite <- H5 in H2_. inversion H2_.
+                  exists NPE. exists sigma.
+                  apply ST_fieldWriteException with (sigma:=sigma) (f:=f) (v:=e).
+                  auto. auto. 
 
-                  assert (argu <> unlabelOpaque t).  apply (H4 t). apply (H4 t). auto. apply v_oid.
-                  (* case for argu <> unlabelOpaque t exception *)
-                  subst. exists NPE. exists (SIGMA s h). 
-              apply ST_MethodCallException with (sigma:=(SIGMA s h)) (v:=argu) (meth:=meth).
+                  rewrite <- H5 in H2_. inversion H2_.
+                  rewrite <- H5 in H2_. inversion H2_.
+                  rewrite <- H5 in H2_. inversion H2_.
+     
+      + destruct  IHhas_type2.  auto. auto. auto. auto. 
+          destruct H4 as [t']. destruct H4 as [sigma']. 
+          exists (FieldWrite t' f e). exists (sigma').   
+          apply ST_fieldWrite1 with (sigma:=sigma) (sigma':=sigma') (f:=f) (e1:=x) (e1':=t') (e2:=e).
+          auto. 
 
-                  subst. inversion H2_.
-                rewrite <- H7 in H2_. inversion H2_.                 rewrite <- H7 in H2_. inversion H2_. 
-            
+          destruct H4 as [t']. destruct H4 as [sigma']. 
+          exists (FieldWrite t' f e). exists (sigma').   
+          apply ST_fieldWrite1 with (sigma:=sigma) (sigma':=sigma') (f:=f) (e1:=x) (e1':=t') (e2:=e).
+          auto. 
 
+(* if *)
+- (*destruct  IHhas_type1; auto.  destruct  IHhas_type2; auto. *)
+  inversion H2. inversion H1. subst. inversion H3. 
+  assert (exists v1, sf id1 = Some v1). 
+  apply Typed_variable with (sigma:=(SIGMA (s) h)) (s:=s) (h:=h) (ct:=CT) 
+                                            (gamma:=Gamma) (x:=id1) (T:=(classTy T)) (lb:=lb) (sf:=sf) (s':=s').
+  auto. auto. auto. auto. 
+  assert (exists v2, sf id2 = Some v2). 
+  apply Typed_variable with (sigma:=(SIGMA (s) h)) (s:=s) (h:=h) (ct:=CT) 
+                                            (gamma:=Gamma) (x:=id2) (T:=(classTy T)) (lb:=lb) (sf:=sf) (s':=s').
+  auto. auto. auto. auto. 
 
+  destruct H19 as [v1].   destruct H20 as [v2].
+  right. inversion H8. inversion H21. destruct H22 with id1 v1. 
+  rewrite <- H27; auto. destruct H22 with id2 v2.  destruct H22 with id1 v1.  
+  rewrite <- H27; auto. rewrite <- H27; auto. rewrite <- H27; auto. 
+  
+  exists s1. exists sigma.
+  apply ST_if_b1 with (sigma:=sigma) (s1:=s1) (s2:=s2) (v1:=v1) (v2:=v2)
+                                (s:=s) (h:=h) (lsf:=lsf) (s':=s') (lb:=lb) (sf:=sf) (id1:=id1) (id2:=id2). 
+  auto. rewrite <- H24 in H4. assumption. auto. auto. auto. subst. auto. 
+  destruct H28.
+  destruct H28.
 
-(*
+  exists s2. exists sigma.
+  apply ST_if_b2 with (sigma:=sigma) (s1:=s1) (s2:=s2) (v1:=v1) (v2:=v2)
+                                (s:=s) (h:=h) (lsf:=lsf) (s':=s') (lb:=lb) (sf:=sf) (id1:=id1) (id2:=id2). 
+  auto. rewrite <- H24 in H4. assumption. auto. auto. auto. intuition. 
+  rewrite -> H25 in H30.  rewrite -> H28 in H30. inversion H30.
+  rewrite -> H25 in H30.  rewrite -> H28 in H30. inversion H30.
+  rewrite -> H25 in H30.  rewrite -> H28 in H30. inversion H30.
+  rewrite -> H25 in H30.  rewrite -> H28 in H30. inversion H30.
 
-(* unlabel opaque*)
-  (* context rule *)
-  | ST_unlabel_opaque1 : forall sigma sigma' e e',
-       e / sigma ==>  e' / sigma' -> 
-      (unlabelOpaque e) / sigma ==> (unlabelOpaque e') / sigma'
-  (* unlabel opaque *)
-  | ST_unlabel_opaque2 : forall sigma v lb l' sigma' s h,
-      sigma = SIGMA s h ->
-      l' = join_label lb (current_label sigma) ->
-      value (v_opa_l v (l lb)) ->
-      (unlabelOpaque ((v_opa_l v (l lb)))) / sigma ==> v / sigma'
-*)
+  exists s2. exists sigma.
+  apply ST_if_b2 with (sigma:=sigma) (s1:=s1) (s2:=s2) (v1:=v1) (v2:=v2)
+                                (s:=s) (h:=h) (lsf:=lsf) (s':=s') (lb:=lb) (sf:=sf) (id1:=id1) (id2:=id2). 
+  auto. rewrite <- H24 in H4. assumption. auto. auto. auto. intuition. 
+  rewrite -> H25 in H29.  rewrite -> H28 in H29. inversion H29.
+  rewrite -> H25 in H29.  rewrite -> H28 in H29. inversion H29.
+  rewrite -> H25 in H29.  rewrite -> H28 in H29. inversion H29.
+  rewrite -> H25 in H29.  rewrite -> H28 in H29. inversion H29.
 
-Theorem preservation : forall t t' T sigma sigma', 
-    gamma |- t \in T ->
-    t / st ==> t' / st' ->
-    gamma |- t' \in T.
+destruct H25. destruct H25. 
 
+destruct H22 with id2 v2.
+  rewrite <- H27.  auto.
+  exists s2. exists sigma.
+  apply ST_if_b2 with (sigma:=sigma) (s1:=s1) (s2:=s2) (v1:=v1) (v2:=v2)
+                                (s:=s) (h:=h) (lsf:=lsf) (s':=s') (lb:=lb) (sf:=sf) (id1:=id1) (id2:=id2). 
+  auto. rewrite <- H24 in H4. assumption. auto. auto. auto. intuition. 
+  rewrite -> H25 in H30. rewrite -> H29 in H30. inversion H30.
+  rewrite -> H25 in H30.  rewrite -> H29 in H30. inversion H30.
+  rewrite -> H25 in H30.  rewrite -> H29 in H30. inversion H30.
+  rewrite -> H25 in H30.  rewrite -> H29 in H30. inversion H30.
 
-Proof.
+destruct H29. destruct H29. 
+  exists s1. exists sigma.
+  apply ST_if_b1 with (sigma:=sigma) (s1:=s1) (s2:=s2) (v1:=v1) (v2:=v2)
+                                (s:=s) (h:=h) (lsf:=lsf) (s':=s') (lb:=lb) (sf:=sf) (id1:=id1) (id2:=id2). 
+  auto. rewrite <- H24 in H4. assumption. auto. auto. auto. rewrite <- H29 in H25. auto.
+
+  exists s2. exists sigma.
+  apply ST_if_b2 with (sigma:=sigma) (s1:=s1) (s2:=s2) (v1:=v1) (v2:=v2)
+                                (s:=s) (h:=h) (lsf:=lsf) (s':=s') (lb:=lb) (sf:=sf) (id1:=id1) (id2:=id2). 
+  auto. rewrite <- H24 in H4. assumption. auto. auto. auto. intuition. 
+  rewrite -> H25 in H30. rewrite -> H29 in H30. inversion H30.
+  rewrite -> H25 in H30.  rewrite -> H29 in H30. inversion H30.
+  rewrite -> H25 in H30.  rewrite -> H29 in H30. inversion H30.
+  rewrite -> H25 in H30.  rewrite -> H29 in H30. inversion H30.
+
+destruct H22 with id2 v2.
+  rewrite <- H27.  auto.
+  exists s2. exists sigma.
+  apply ST_if_b2 with (sigma:=sigma) (s1:=s1) (s2:=s2) (v1:=v1) (v2:=v2)
+                                (s:=s) (h:=h) (lsf:=lsf) (s':=s') (lb:=lb) (sf:=sf) (id1:=id1) (id2:=id2). 
+  auto. rewrite <- H24 in H4. assumption. auto. auto. auto. intuition. 
+  rewrite -> H25 in H29. rewrite -> H28 in H29. inversion H29.
+  rewrite -> H25 in H29. rewrite -> H28 in H29. inversion H29.
+  rewrite -> H25 in H29. rewrite -> H28 in H29. inversion H29.
+  rewrite -> H25 in H29. rewrite -> H28 in H29. inversion H29.
+
+destruct H28. destruct H28. 
+  exists s2. exists sigma.
+  apply ST_if_b2 with (sigma:=sigma) (s1:=s1) (s2:=s2) (v1:=v1) (v2:=v2)
+                                (s:=s) (h:=h) (lsf:=lsf) (s':=s') (lb:=lb) (sf:=sf) (id1:=id1) (id2:=id2). 
+  auto. rewrite <- H24 in H4. assumption. auto. auto. auto. intuition.   
+  rewrite -> H25 in H30. rewrite -> H28 in H30. inversion H30.
+  rewrite -> H25 in H30. rewrite -> H28 in H30. inversion H30.
+  rewrite -> H25 in H30. rewrite -> H28 in H30. inversion H30.
+  rewrite -> H25 in H30. rewrite -> H28 in H30. inversion H30.
+
+exists s1. exists sigma.
+  apply ST_if_b1 with (sigma:=sigma) (s1:=s1) (s2:=s2) (v1:=v1) (v2:=v2)
+                                (s:=s) (h:=h) (lsf:=lsf) (s':=s') (lb:=lb) (sf:=sf) (id1:=id1) (id2:=id2). 
+  auto. rewrite <- H24 in H4. assumption. auto. auto. auto. rewrite -> H25. rewrite -> H28. auto. 
+
+(* sequence *)
+- right. destruct IHhas_type1. auto. auto. auto.
+   exists e2. exists sigma. 
+   apply ST_seq2 with (sigma:=sigma) (v:=e1) (s:=e2); auto.
+  
+  destruct H2 as [t']. destruct H2 as [sigma'].
+  exists (Sequence t' e2). exists sigma. 
+   apply ST_seq1 with (sigma:=sigma) (s1:=e1) (s2:=e2) (s1':=t'); auto.
+
+(* return e *)
+- right. destruct IHhas_type. auto. auto. auto. 
+  assert (exists lsf s', s = cons lsf s'). 
+  apply stack_not_nil with (sigma:=sigma) (gamma:=Gamma) (CT:=CT) (s:=s) (h:=h).
+  auto. auto. auto.
+  destruct H5 as [lsf]. destruct H5 as [s'].
+  remember (join_label (get_current_label s) (get_current_label s')) as l'.
+  remember (update_current_label s' l' ) as s''.
+  remember (SIGMA s'' h) as sigma'.
+  exists e. exists sigma'.
+  apply ST_return2 with (sigma:=sigma) (sigma':=sigma') (v:=e)
+                                    (s:=s) (s':=s') (s'':=s'') (h:=h) (lsf:=lsf) (l':=l').
+  auto. auto. auto. auto. auto. auto. 
+
+  destruct H4 as [t']. destruct H4 as [sigma'].
+  exists (Return t'). exists sigma'. 
+  apply ST_return1 with (sigma:=sigma) (sigma':=sigma') (e:=e) (e':=t'). auto.
+
+(* ObjId o *)
+- left. apply v_oid. 
+
+(* v_l *)
+- left. apply v_labeled. 
+
+(* v_opl_l *)
+- left. apply v_opa_labeled.
 Qed.
+
+(* reduction preserve well-form of stack and heap *)
+
+
+
+(* reduction preserve typing *)
+
+Theorem preservation : forall t t' T  sigma sigma' gamma CT s h h', 
+    sigma = SIGMA s h ->  wfe_heap CT gamma h -> wfe_stack CT gamma h s -> 
+    has_type CT gamma h t T -> 
+    t / sigma ==> t' / sigma' ->
+    exists T', has_type CT gamma h' t' T'.
+Proof with auto.
+    intros. induction H3.
+- (* Tvar *)
+   inversion H2. inversion H1. rewrite -> H15 in H11. inversion H11. 
+   inversion H16. 
+Qed.
+
+
 
 
 
